\documentclass{assignment}
\title{5370 Midterm}

\begin{document}


\textbf{4.} Problem 2.10b in the text:\\
\begin{align*}
  H(X) & = -\alpha\log\alpha - (1 - \alpha)\log (1- \alpha) + \alpha H(X_1) + (1 - \alpha) H(X_2)
\end{align*}
Maximize over $\alpha$ to show that $2^{H(X)}\leq 2^{H(X_1)} + 2^{H(X_2) }$ and interpret using the notion that $2^{H(X)}$ is the effective alphabet size.\\

\textbf{Solution:} \\
\begin{align*}
  \df{d}{d\alpha} H(X)
  & = \df{d}{d\alpha}\left[ -\alpha\log\alpha - (1 - \alpha)\log (1- \alpha) + \alpha H(X_1) + (1 - \alpha) H(X_2)\right]
    = 0 \\
  & = -\left(\log \alpha + \alpha \df{1}{\alpha}\right) - \left( - \log(1-\alpha) - (1-\alpha)\df{1}{1-\alpha}\right)
      + H(X_1) - H(X_2)\\
  & =  -\log\alpha - 1 + \log(1-\alpha) + 1 + H(X_1) - H(X_2) \\
  & =  \log(1-\alpha) - \log\alpha + H(X_1) - H(X_2) \\
  & = \log\left( \df{1 -\alpha}{\alpha} \right) + H(X_1) - H(X_2) = 0\\
  \Rightarrow \log\left( \df{1 -\alpha}{\alpha} \right) & = H(X_2) - H(X_1) \\
  \df{1 - \alpha}{\alpha} & = 2^{H(X_2) - H(X_1)} \\
  1 & = \alpha 2^{H(X_2) - H(X_1)} + \alpha\\
  1 & = \alpha \left( 2^{H(X_2) - H(X_1)} + 1 \right) \\
  \alpha & = \df{1}{2^{H(X_2) - H(X_1)} + 1} = \df{1}{K + 1} \\
  \shortintertext{where:}
  K & = 2^{H(X_2) - H(X_1)}
\end{align*}
So we have:
\begin{align*}
  1 - \alpha & = 1 - \df{1}{K + 1} = \df{K}{K + 1} \\
  H(X) & = - \df{1}{K + 1} \log\left( \df{1}{K + 1} \right) - \df{K}{K + 1}\log\left( \df{K}{K + 1} \right)
           + \df{1}{K + 1} H(X_1) + \df{K}{K + 1}H(X_2) \\
             & = \df{\log(K + 1) - K\log\left( \df{K}{K + 1} \right) + H(X_1) + K H(X_2)}{K + 1} \\
             & = \df{\log(K + 1) - K\log(K) + K\log(K+1) + H(X_1) + K H(X_2)}{K + 1} \\
             & = \df{H(X_1) +K H(X_2) - K\log(K)}{K+1} + \log(K+1) \\
  \shortintertext{let $a=H(X_1)$, $b=H(X_2)$}
  H(X) & = \df{a +2^{b - a} b - 2^{b - a}\log(2^{b - a})}{2^{b - a}+1} + \log(2^{b - a}+1)
             % & = \df{\log(K + 1) + K\log\left( \df{K + 1}{K} \right) + H(X_1) + K H(X_2)}{K + 1} \\
             % & = \df{\log(K + 1) + K\log\left( 1 + \df{1}{K} \right) + H(X_1) + KH(X_2)}{K + 1}
\end{align*}

% \begin{align*}
%   \shortintertext{Since:}
%   \log (a + b) & = \log(a * (1 + b/a)) \\
%   \shortintertext{We have:}
%   \log(K + 1) & = \log\left(K * \left(1 + \df{1}{K}\right)\right)\\
%                & = K + \log\left(1 + \df{1}{K}\right) \\
% \end{align*}
% So,
% \begin{align*}
%   H(X) & = \df{K + \log\left(1 + \df{1}{K}\right)
%          + K\log\left( 1 + \df{1}{K}
%          \right) + H(X_1) + KH(X_2)}{K + 1} \\
%        & = \df{K + \log\left(1 + \df{1}{K}\right)\left( 1 +  K\right)
%          + H(X_1) + KH(X_2)}{K + 1} \\
%        & = \df{K + H(X_1) + KH(X_2)}{K + 1}
%            + \log\left(\df{K + 1}{K}\right)
% \end{align*}
\end{document}
